tactics for rule removal

Code/Examples/MapRuleRemoval.v
@@ -59,16 +59,24 @@ Definition map_afs :=
 (** The polynomials *)
 Definition map_fun_poly f : poly ∙ (arity map_afs f) :=
   match f with
-  | TNil => P_base (P_const 3)
-  | TCons => λP λP (P_base (P_const 3))
+  | TNil => P_base (P_const 2)
+  | TCons =>
+    λP let y0 := P_var (Vz) in
+    λP let y1 := P_var (Vs Vz) in
+    P_base (P_const 3 + y0 + y1)
   | TMap =>
     λP let y0 := P_var Vz in
     λP let G1 := P_var (Vs Vz) in
-    P_base (P_const 3 * y0 + G1 ·P y0 + P_const 3 * y0 * G1 ·P y0)
+    P_base (P_const 3 + P_const 3 * y0 + G1 ·P y0 + P_const 3 * y0 * G1 ·P y0)
   end.
 
 (** Strong normalization *)
-Definition map_isSN : isSN map_afs.
+Theorem map_isSN : isSN map_afs.
 Proof.
-  solve_poly_SN map_fun_poly.
+  certificate_SN.
+  rule_removal_certificate (0 :: nil).
+  { poly_certificate map_fun_poly. }
+  rule_removal_certificate (0 :: nil).
+  { poly_certificate map_fun_poly. }
+  empty_certificate.
 Qed.
