Code/TerminationTechniques.v
@@ -2,3 +2,4 @@ Require Export Nijn.TerminationTechniques.RuleRemoval.
 Require Export Nijn.TerminationTechniques.PolynomialMethod.
 Require Export Nijn.TerminationTechniques.NoRules.
 Require Export Nijn.TerminationTechniques.Certificate.
+Require Export Nijn.TerminationTechniques.CertificateTactics.
