Code/TerminationTechniques/RuleRemoval/RuleRemovalTactics.v
@@ -1,0 +1,4 @@
+Require Import Nijn.TerminationTechniques.RuleRemoval.RuleSelector.
+Require Import Nijn.TerminationTechniques.RuleRemoval.RuleRemovalTheorem.
+
+Ltac remove_rules 
